Main.lean
@@ -1,4 +1,4 @@
-import Is0
+import Risc0
 
 def main : IO Unit :=
   return ()
